make compile. proofs still incomplete

examples/lambda/Lambda.hs
@@ -8,11 +8,15 @@ data Expr
   | Lam Name Expr
   | App Expr Expr
 
+
+maxName :: Name -> [Name] -> Name
+maxName n ns = foldr max n ns
+
 maxVar :: Expr -> Int
 maxVar (Var n) = n
-maxVar (Let n e1 e2) = maximum [n, maxVar e1, maxVar e2]
-maxVar (Lam n e) = maximum [n, maxVar e]
-maxVar (App e1 e2) = maximum [maxVar e1, maxVar e2]
+maxVar (Let n e1 e2) = maxName n [maxVar e1, maxVar e2]
+maxVar (Lam n e) = maxName  n [maxVar e]
+maxVar (App e1 e2) = maxName (maxVar e1) [maxVar e2]
 
 fresh :: Expr -> Int
 fresh e = 1 + maxVar e
@@ -24,4 +28,3 @@ anf (Lam n body) = Lam n (anf body)
 anf (App f (Var n)) = App (anf f) (Var n)
 anf (App f e) = Let v (anf e) (App (anf f) (Var v))
   where v = fresh f
-
