examples/lambda/Proofs.v
@@ -3,27 +3,33 @@ Require Import Lambda.
 
 Definition isVal (e : Expr) : Prop :=
   match e with
-    | Mk_Var _ => True
-    | Mk_Lam _ _ => True
+    | Var _ => True
+    | Lam _ _ => True
     | _ => False
   end.
 
+Definition rename : Name -> Name -> Expr -> Expr :=
+  fix rename v w body
+        := match body with
+             | Var v' => Var (if v == v' then w else v')
+             | Lam v' e => Lam v' (if v == v' then e else rename v w e)
+             | App e1 e2 => App (rename v w e1) (rename v w e2)
+             | Let v' rhs body => Let v' (rename v w rhs) (if v == v'
+                                                          then body
+                                                          else rename v w body)
+           end.
 
-Fixpoint rename v w body := match body with
-  | Mk_Var v' => Mk_Var (if v == v' then w else v')
-  | Mk_Lam v' e => Mk_Lam v' (if v == v' then e else rename v w e)
-  | Mk_App e1 e2 => Mk_App (rename v w e1)  (rename v w e2)
-  | Mk_Let v' rhs body => Mk_Let v' (rename v w rhs) (if v == v' then body else rename v w body)
-end.
 
-Fixpoint depth e := match e with 
-  | Mk_Var v' => 0
-  | Mk_Lam v' e => S (depth e)
-  | Mk_App e1 e2 =>
+
+Fixpoint depth e := match e with
+  | Var v' => 0
+  | Lam v' e => S (depth e)
+  | App e1 e2 =>
     PeanoNat.Nat.max (S (depth e1)) (S (depth e2))
-  | Mk_Let v' rhs body =>
+  | Let v' rhs body =>
     PeanoNat.Nat.max (S (depth rhs)) (S (depth body))
 end.
+
 
 Lemma depth_rename : forall v w e,
     depth (rename v w e) = depth e.
@@ -32,11 +38,11 @@ Proof.
   induction e.
   * auto.
   * simpl.
-    destruct (negb (v =? n)%Z).
+    destruct (v == n).
     + rewrite IHe1. auto.
     + rewrite IHe1. rewrite IHe2. auto.
   * simpl.
-    destruct (negb (v =? n)%Z).
+    destruct (v == n).
     + auto.
     + rewrite IHe. auto.
   * simpl.
@@ -49,16 +55,16 @@ Require Import Recdef.
 
 Function subst v arg body {measure depth body} :=
   match body with
-  | Mk_Var v' => if v == v' then arg else Mk_Var v'
-  | Mk_Lam v' e => if v == v' then Mk_Lam v' e else
+  | Var v' => if v == v' then arg else Var v'
+  | Lam v' e => if v == v' then Lam v' e else
                     let f := fresh e in
-                    Mk_Lam f (subst v arg (rename v' v e))
-  | Mk_App e1 e2 => Mk_App (subst v arg e1)  (subst v arg e2)
-  | Mk_Let v' rhs body =>
+                    Lam f (subst v arg (rename v' v e))
+  | App e1 e2 => App (subst v arg e1)  (subst v arg e2)
+  | Let v' rhs body =>
     let v'' := fresh body in
     let rhs' := subst v arg rhs in
     let body' := subst v arg (rename v' v'' body) in
-    Mk_Let v' rhs' body'
+    Let v' rhs' body'
   end.
 Proof.
   all: intros; simpl;
@@ -68,49 +74,49 @@ Qed.
 Inductive small_step : Expr -> Expr -> Prop :=
 | ss_beta : forall v body arg,
     isVal arg ->
-    small_step (Mk_App (Mk_Lam v body) arg) (subst v arg body)
+    small_step (App (Lam v body) arg) (subst v arg body)
 | ss_let: forall v body rhs ,
     isVal rhs ->
-    small_step (Mk_Let v rhs body) (subst v rhs body)
+    small_step (Let v rhs body) (subst v rhs body)
 | ss_let_search: forall v body rhs rhs',
     small_step rhs rhs' ->
-    small_step (Mk_Let v rhs body) (Mk_Let v rhs' body)
+    small_step (Let v rhs body) (Let v rhs' body)
 | ss_app_search : forall m m' n,
     small_step m m' ->
-    small_step (Mk_App m n) (Mk_App m' n)
+    small_step (App m n) (App m' n)
 | ss_app_val: forall m n n',
     isVal m ->
     small_step n n' ->
-    small_step (Mk_App m n) (Mk_App m n').
+    small_step (App m n) (App m n').
 
 
 Fixpoint small_step_fun (t : Expr) : option Expr :=
   match t with
-  | Mk_App t1 t2 => match t1 with
-                | Mk_Lam v t3 =>
+  | App t1 t2 => match t1 with
+                | Lam v t3 =>
                   match small_step_fun t2 with
-                  | Some t2' => Some (Mk_App t1 t2')
+                  | Some t2' => Some (App t1 t2')
                   | _ => match t2 with
-                        | Mk_App _ _ => None
+                        | App _ _ => None
                         | _ => Some (subst v t2 t3)
                         end
                   end
-                | Mk_Var i =>
+                | Var i =>
                   match small_step_fun t2 with
-                    | Some t2' => Some (Mk_App t1 t2')
+                    | Some t2' => Some (App t1 t2')
                     | _ => None
                     end
                 | _ => match (small_step_fun t1) with
-                      | Some t1' => Some (Mk_App t1' t2)
+                      | Some t1' => Some (App t1' t2)
                       | _ => None
                       end
                    end
-  | Mk_Let v t1 t2 =>
+  | Let v t1 t2 =>
     match t1 with
-      | Mk_Var _ => Some (subst v t1 t2)
-      | Mk_Lam _ _ => Some (subst v t1 t2)
+      | Var _ => Some (subst v t1 t2)
+      | Lam _ _ => Some (subst v t1 t2)
       | _ => match (small_step_fun t1) with
-            | Some t1' => Some (Mk_Let v t1' t2)
+            | Some t1' => Some (Let v t1' t2)
             | _ => None
             end
     end
@@ -122,7 +128,7 @@ Lemma isVal_not_step: forall n,
 Proof.
   intros []; auto;
   intros H; inversion H.
-Qed.  
+Qed.
 
 
 Lemma small_step_small_step_fun : forall m m',
@@ -144,27 +150,27 @@ Proof.
       * simpl in IHsmall_step.
         simpl.
         destruct rhs0; auto.
-        -- destruct (small_step_fun (Mk_Let n rhs0_1 rhs0_2)).
+        -- destruct (small_step_fun (Let n rhs0_1 rhs0_2)).
            inversion IHsmall_step. auto.
         -- inversion IHsmall_step.
-      * destruct (small_step_fun (Mk_App rhs0_1 rhs0_2));
+      * destruct (small_step_fun (App rhs0_1 rhs0_2));
           inversion IHsmall_step; auto.
       * simpl in IHsmall_step.
-        simpl.        
+        simpl.
         destruct rhs0.
         -- inversion IHsmall_step. auto.
-        -- destruct (small_step_fun (Mk_Let n rhs0_1 rhs0_2)).
+        -- destruct (small_step_fun (Let n rhs0_1 rhs0_2)).
            inversion IHsmall_step. auto.
         -- inversion IHsmall_step.
         -- inversion IHsmall_step. auto.
-        -- destruct (small_step_fun (Mk_App rhs0_1 rhs0_2));
+        -- destruct (small_step_fun (App rhs0_1 rhs0_2));
              inversion IHsmall_step; auto.
         - simpl in IHsmall_step.
            simpl.
            destruct m; try solve [inversion H0].
-           ++ destruct (small_step_fun (Mk_Let n0 m1 m2));
+           ++ destruct (small_step_fun (Let n0 m1 m2));
                 inversion IHsmall_step; subst; auto.
-           ++ destruct (small_step_fun (Mk_App m1 m2));
+           ++ destruct (small_step_fun (App m1 m2));
                 inversion IHsmall_step; auto.
         -- simpl in IHsmall_step.
            simpl.
@@ -182,10 +188,10 @@ Proof.
                  simpl.
            ++ destruct m1; inversion IHsmall_step; auto.
               ** destruct (small_step_fun
-                             (Mk_Let n1 m1_1 m1_2));
+                             (Let n1 m1_1 m1_2));
                    inversion IHsmall_step; auto.
               ** destruct (small_step_fun
-                             (Mk_App m1_1 m1_2));
+                             (App m1_1 m1_2));
                    inversion IHsmall_step; auto.
         + simpl. simpl in IHsmall_step.
               intuition.
@@ -204,43 +210,43 @@ Notation "R ^*" := (rtc R) (at level 1, format "R ^*").
 
 Definition nf (x: Expr): Prop := ~ exists y, small_step x y.
 
+(*
 Inductive beta_equiv : Expr -> Expr -> Prop :=
 | be_refl: forall x, beta_equiv x y
-| be_
 | be_Step: forall v x y,
-    beta_equiv (Mk_Let v x y) (Mk_App (Mk_Lam v y) x)
-               
-| be_Var : forall v, beta_equiv (Mk_Var v) (Mk_Var v)
+    beta_equiv (Let v x y) (App (Lam v y) x)
+
+| be_Var : forall v, beta_equiv (Var v) (Var v)
 | be_Let: forall v x1 x2 y1 y2,
     beta_equiv x1 x2 -> beta_equiv y1 y2 ->
-    beta_equiv (Mk_Let v x1 y1) (Mk_Let v x2 y2)
+    beta_equiv (Let v x1 y1) (Let v x2 y2)
 | be_App: forall x1 x2 y1 y2,
     beta_equiv x1 x2 -> beta_equiv y1 y2 ->
-    beta_equiv (Mk_App x1 y1) (Mk_App x2 y2)
+    beta_equiv (App x1 y1) (App x2 y2)
 | be_Lam: forall v x1 x2,
     beta_equiv x1 x2 ->
-    beta_equiv (Mk_Lam v x1) (Mk_Lam v x2).
-                           
+    beta_equiv (Lam v x1) (Lam v x2).
+
 | ss_beta : forall v body arg,
     isVal arg ->
-    small_step (Mk_App (Mk_Lam v body) arg) (subst v arg body)
+    small_step (App (Lam v body) arg) (subst v arg body)
 | ss_let: forall v body rhs ,
     isVal rhs ->
-    small_step (Mk_Let v rhs body) (subst v rhs body)
-
-(* 
+    small_step (Let v rhs body) (subst v rhs body)
+*)
+(*
 Let x y z ==  App (Lam x z)  y
 
 
 
     Lam x (App x (Lam y y)) is nf
-anf (Lam x (App x (Lam y y))) = 
+anf (Lam x (App x (Lam y y))) =
      Lam x (Let z = (Lam y y) in x z)
 *)
+(*
 Theorem anf_correct: forall x y,
     small_step^* x y -> nf y ->
     small_step^* (anf x) y' /\ R y y'.
 Proof.
   intros x y Hs Hn.
-  
-  
+*)
